---
layout: post
title:  "An Introduction to Abstract Algebra (Part 6)"
date:   2016-04-15
categories: Abstract Algebra
---

Welcome to the sixth post on my abstract algebra series. Today Iâ€™ll go over cyclic groups.

Let G be a group. G is cyclic if there exists a $$g \in G$$ such that $$G = \{g^n : n \in \mathbb{Z}\}$$. This property is denoted $$G = <g>$$ and we say that G is generated by g.

For example, $$(\mathbb{Z}, +) = <1>$$ ($$\mathbb{Z}$$ is the group of all integers with addition as the group operation) and $$(\mathbb{Z}/n\mathbb{Z}, +) = <1>$$ ($$\mathbb{Z}/n\mathbb{Z}$$ is the group of integers modulo n, ie integers from 1 to n-1, with addition as the group operation).

A note on notation: when we are working with $$\mathbb{Z}/n\mathbb{Z}$$ all integers (and variables) are modulo n. This is comonly denoted by placing a bar on top of numbers and variables (eg, $$\bar{x}, \bar{2}$$ are both modulo n) but for simplicity I will not use this notation unless not using it would result in ambiguity $$ a\vert b$$ means that a divides b, and (a, b) denotes the greater common divisor of a and b.

Proposition: the order of an element is equal to the size of the group it generates. If $$H = <x>$$ is infinite then $$x^i = x^j$$ if and only if i = j, hence x has infinite order. If $$H = <x>$$ is finite and $$|H| = n$$ then $$H = \{1, x, ..., x^{n-1}\}$$, so x has order n.

Theorem: let H be cyclic generated by x, then (1) if the order of x is infinite then $$H \cong \mathbb{Z}$$ (2) if $$\vert x\vert = n \in \mathbb{Z}_{> 0}$$ then $$H \cong \mathbb{Z}/n\mathbb{Z}$$.

Proof: (1) Let $$f: \mathbb{Z} \rightarrow H$$ be a homomorphism that sends $$i \mapsto x^i$$. Since $$f(i+j) = x^{i+j} = x^i \cdot x^j = f(i)\cdot f(j)$$ f is well defined. Since $$f(i) = 1$$ if and only if $$x^i = 0$$ if and only if i = 0 then f is injective. Finally since $$H = \{x^n : n \in \mathbb{Z}\} = f(\mathbb{Z})$$, f is surjective. This completes the proof for part 1.
(2) let $$f : \mathbb{Z}/n\mathbb{Z} \rightarrow H$$ be a homomorphism that sends $$i \mapsto x^i$$. If i = j then $$x^i = x^j$$ since if i = j  then $$n | i-j = n \cdot k, x^{i+j} = x^ix^j = x^n = 1$$. We can also see that $$f(i+j) = x^{i+j} = x^ix^j = f(i)+f(j)$$ so this homomorphism is well defined. $$f(i) = 1$$ if and only if $$x^i = 1$$ where i = qn+r and $$0 \leq r < n$$. Hence $$x^i = x^{qn+r} = (x^n)^q\cdot x^r = 1$$ so r = 0 and i = 0, hence f is injective. Since $$H = \{1, x, ..., x^{n-1}\} = f(\mathbb{Z}/n\mathbb{Z})$$ f is surjective. Thiscompletes the proof for part 2.

Remark: if H and G are cyclic, $$H \cong G$$ if and only if $$\vert H\vert = \vert G\vert$$

Proposition: (1) Let $$H = <x>$$ be finite, then for all $$a \in \mathbb{Z}-{0}$$ (all integers except 0) $$x^a$$ has finite order. (2) Let $$H = <x>$$ be finite with $$|H| = n$$ then for all $$a \in \mathbb{Z}$$ $$x^a$$ has order $$\frac{n}{(n,a)}$$

Proof: (1) $$(x^a)^m = x^{am} = 1$$ if and only if am = 0 if and only if m = 0, so $$x^a$$ has infinite order.
(2) $$(x^a)^m = x^{am} = 1$$ if and only if am = 0 mod n if and only if $$n| am$$. Let d = (n,a) where $$n = d \cdot k, a = d \cdot l$$ and (k,l) = 1. From that it follows that $$n | am$$ if $$dk | dlm$$ if and only if $$k | lm$$ if and only if $$k | m$$, hence the order of $$x^a$$ is k = $$\frac{n}{(n, a)}$$.

Proposition: (1) if $$H = <x>$$ is finite, with $$a, b \in \mathbb{Z}$$, $$<x^a> = <x^b$$ if and only if $$|a| = |b|$$ (2) If $$H = <x>$$ is finite and $$|H| = n$$ with $$a, b \in \mathbb{Z}$$, $$<x^a> = <x^b$$ if and only if (a,n) = (b,n).

Proof: (1) $$<x^a = \{ x^n : n \in \mathbb{Z}\}$$. If $$x^b \in \{ x^n :n \in \mathbb{Z}\}, x^b = x^{am} = b = am$$ so $$a\vert b$$. Similarly $$b \vert a$$ so $$\vert b \vert = \vert a\vert$$. Conversely if $$\vert a\vert = \vert b\vert$$ then $$b = \pm a$$ so $$x^b = x^a$$ or $$x^{-a}$$ and $$<x^a> = <x^{-a}>$$.
(2) $$<x^a> = <x^b>$$ so $$\vert x^a\vert = \vert x^b\vert$$ so $$\frac{n}{(n,a)} = \frac{n}{(n,b)}$$ so (n,a) = (n,b). Conversely assume (n,a) = (n,b) = d we have a = kd, so $$x^a \in <x^d>$$ which means $$<x^d$$ and $$<x^a> \leq <x^d>$$. Since $$\vert <x^a\vert = \frac{n}{d}, \vert <x^d\vert = \frac{n}{(n,d)} = \frac{n}{d}$$ so $$<x^a> = <x^d>$$. Similarly $$<x^b = <x^d> = <x^a>$$.

Stay tuned for a post on equivalence class, quotients, normal groups and Lagrange's theorem!
