---
layout: post
title:  "An Introduction to Abstract Algebra (Part 10)"
date:   2016-04-23
categories: Abstract Algebra
---

Welcome to the tenth post on my abstract algebra series. Today Iâ€™ll cover the alternating group.

Let $$\sigma \in S_n$$, the number of inversions of $$\sigma$$ is $$\vert \{(i,j); 0 \leq i < j < n; \sigma(j) < \sigma(i)\} \vert$$ = inv($$\sigma$$). For example (1,2) has 1 inversion, $$j > i, (i,j)$$ has $$2(j-i-1)+1$$ inversions, (1,2,3) has 2 inversions.

Let $$\sigma \in S_n$$ we define the sign of $$\sigma$$ to be $$(-1)^{inv(\sigma)} = \varepsilon(\sigma) \in {1, -1}$$. For example $$\varepsilon((i j)) = -1, \varepsilon((1 2 3)) = 1, \varepsilon(1) = 1$$.

Proposition: Let $$\Delta = \prod_{i < j}(x_i-x_j)$$. Let $$\sigma \in S_n$$ and let $$\sigma(\Delta) = \prod_{i<j}(x_{\sigma(i)}-x_{\sigma(j)})$$, then $$\sigma(\Delta) = \varepsilon(\sigma) \cdot \Delta$$

Proof: $$\sigma(\Delta) = \prod_{i < j}(x_{\sigma(i)} - x_{\sigma(j)}) = \prod_{\sigma(i)<\sigma(j)}((x_{\sigma(i)}-x_{\sigma(j)})(-1)^{\varepsilon_{ij}})$$ where $$\varepsilon_{ij} = 0$$ if there is no inversion or 1 if there is inversion. This expression is therefore equal to $$(-1)^{inv(\sigma)}\prod_{k <l}(x_k-x_l) = \varepsilon(\sigma)\cdot \Delta$$

Proposition: $$\sigma : S_n \rightarrow \{1, -1\}$$ is a group morphism.

Proof: let $$\tau, \sigma \in S_n$$. Then $$\tau \sigma(\Delta) = \varepsilon(\tau \sigma)\Delta = $$ $$\prod_{i<j}(x_{\tau(\sigma(i))}-x_{\tau(\sigma(j))}) =$$ $$\prod_{\sigma(i)<\sigma(j)}(x_{\tau(\sigma(i))}-x_{\tau(\sigma(j))}) =$$ $$(-1)^{inv(\sigma)} \prod_{k<l}(x_{\tau(k)}-x_{\tau(l)}) = $$ $$ \varepsilon(\sigma)\tau(\Delta) = $$ $$ \varepsilon(\sigma)\varepsilon(\tau)\Delta$$ so $$\varepsilon(\tau \sigma) = \varepsilon(\tau)\varepsilon(\sigma)$$

Alternating group ($$A_n$$): the alternating group is defined as $$A_n =$$ ker($$\varepsilon) \unlhd S_n$$. For $$n \geq 2$$ by the first isomorphism theorem $$\{1, -1\} \cong S_n/A_n$$ and by Lagrange $$\vert A_n \vert = \frac{\vert S_n \vert}{2} = \frac{n!}{2}$$. For example: $$A_1 = S_1 = \{1\}, A_2 = \{1\}, A_3 = <(1 2 3)>$$

Proposition: if $$\gamma \in S_n$$ is a k cycle, then $$\varepsilon(\gamma) = (-1)^{k-1}$$

Proof: let's consider $$\gamma = (0 1 ... k-1) = (k-1 0)(k-2 0)...(2 0)(1 0)$$ $$\varepsilon(\gamma) = (-1)^{k-1}, \gamma = (a_0 ... a_{k-1})$$, where $$\sigma \in S_n$$. Claim: $$\sigma \gamma \sigma^{-1} = (\sigma(a_0)...\sigma(a_{k-1})), 0 < i < k-1$$ $$\sigma \gamma \sigma^{-1}(\sigma(a_i)) = \sigma \gamma(a_i) = \sigma(a_{i+1})$$ $$ \sigma \gamma \sigma^{-1} (\sigma(a_{k-1})) = \sigma \gamma (a_{k-1}) = \sigma(a_0)$$ Let $$x \not\in \{\sigma(a_i), 0 \leq i < k\}$$ then $$\sigma \gamma \sigma^{-1}(x) = \sigma(\sigma^{-1}(x)) = x$$ so$$ \sigma^{-1}(x) \not\in \{a_i, 0 \leq i < k\}$$. Let $$\sigma(i) = a_i, 0 \leq i < k$$. By induction $$l \geq k =$$ min$$\{0 ... n-1\}\backslash  \{\sigma(i) j < l\},$$ by construction $$\sigma$$ is injective so $$\sigma \in S_n$$ $$\sigma(0 ... k-1)\sigma^{-1} = (\sigma(0)... \sigma(k-1)) = (a_0 ... a_{k-1}) = \gamma$$ $$ \varepsilon(\gamma) = \varepsilon(\sigma(0 ... k-1)\sigma^{-1}) = \varepsilon(\sigma)\varepsilon((0 ... k-1))\epsilon(\sigma) = (-1)^{k-1}$$

From above it follows that $$A_4 = \{$$1, (1 2 3), (1 3 2), (1 2)(3 4), (1 2 4), (1 4 2), (1 3 4), (1 4 3), (2 3 4), (2 4 3), (1 3)(2 4), (1 4)(2 3)$$\}$$. Note that $$A_4$$ is not simple.

Theorem: $$A_n$$ is simple if $$n \geq 5$$. $$A_n$$ is generated by 3 cycles.

Stay tuned for a post on group actions!
